translate HistoryLengthInvariant to TLS states

ironfleet/src/Dafny/Distributed/Protocol/Lock/PerformanceProof/Invariants.i.dfy
@@ -1,8 +1,8 @@
 include "../../../Common/Framework/Environment.s.dfy"
-include "../../Lock/RefinementProof/DistributedSystem.i.dfy"
+include "TimestampedGLS.i.dfy"
 
 module Invariants_i {
-    import opened DistributedSystem_i
+    import opened TimestampedGLS_i
     import opened Environment_s
 
 
@@ -11,10 +11,10 @@ module Invariants_i {
 *****************************************************************************************/
 
 
-predicate HistoryLengthInvariant(config:ConcreteConfiguration, gls:GLS_State)
+predicate HistoryLengthInvariant(config:ConcreteConfiguration, gls:TimestampedGLS_State)
     requires |gls.history| > 0;
-    requires forall ep :: ep in gls.ls.servers <==> ep in config;
-    requires forall ep | ep in gls.ls.servers :: gls.ls.servers[ep].config == config;
+    requires forall ep :: ep in gls.tls.t_servers <==> ep in config;
+    requires forall ep | ep in gls.tls.t_servers :: gls.tls.t_servers[ep].v.config == config;
 {
     && AtMostOneLockHolder(config, gls)
     && NoLockHolderImpliesOneTransferMessageInFlight(config, gls)
@@ -27,304 +27,304 @@ predicate HistoryLengthInvariant(config:ConcreteConfiguration, gls:GLS_State)
 
 
 
-predicate AtMostOneLockHolder(config:ConcreteConfiguration, gls:GLS_State) 
-    requires forall ep :: ep in gls.ls.servers <==> ep in config;
-    requires forall ep | ep in gls.ls.servers :: gls.ls.servers[ep].config == config;
+predicate AtMostOneLockHolder(config:ConcreteConfiguration, gls:TimestampedGLS_State) 
+    requires forall ep :: ep in gls.tls.t_servers <==> ep in config;
+    requires forall ep | ep in gls.tls.t_servers :: gls.tls.t_servers[ep].v.config == config;
 {
-    forall ep1, ep2 | ep1 in config && ep2 in config :: gls.ls.servers[ep1].held && gls.ls.servers[ep2].held ==> ep1 == ep2
+    forall ep1, ep2 | ep1 in config && ep2 in config :: gls.tls.t_servers[ep1].v.held && gls.tls.t_servers[ep2].v.held ==> ep1 == ep2
 }   
 
-predicate NoLockHolder(config:ConcreteConfiguration, gls:GLS_State) 
-    requires forall ep :: ep in gls.ls.servers <==> ep in config;
-    requires forall ep | ep in gls.ls.servers :: gls.ls.servers[ep].config == config;
+predicate NoLockHolder(config:ConcreteConfiguration, gls:TimestampedGLS_State) 
+    requires forall ep :: ep in gls.tls.t_servers <==> ep in config;
+    requires forall ep | ep in gls.tls.t_servers :: gls.tls.t_servers[ep].v.config == config;
 {
-    forall ep | ep in config :: !gls.ls.servers[ep].held
+    forall ep | ep in config :: !gls.tls.t_servers[ep].v.held
 }
 
 
-predicate IsInFlightTransferMessage(config:ConcreteConfiguration, gls:GLS_State, p:LPacket<EndPoint, LockMessage>) 
-    requires forall ep :: ep in gls.ls.servers <==> ep in config;
-    requires forall ep | ep in gls.ls.servers :: gls.ls.servers[ep].config == config;
+predicate IsInFlightTransferMessage(config:ConcreteConfiguration, gls:TimestampedGLS_State, p:LPacket<EndPoint, TimestampedType<LockMessage>>) 
+    requires forall ep :: ep in gls.tls.t_servers <==> ep in config;
+    requires forall ep | ep in gls.tls.t_servers :: gls.tls.t_servers[ep].v.config == config;
 {
-    && p in gls.ls.environment.sentPackets  
+    && p in gls.tls.t_environment.sentPackets  
     && p.dst in config 
     && p.src in config 
-    && p.msg.Transfer?
-    && p.msg.transfer_epoch > gls.ls.servers[p.dst].epoch
+    && p.msg.v.Transfer?
+    && p.msg.v.transfer_epoch > gls.tls.t_servers[p.dst].v.epoch
 }
 
-predicate OneTransferMessageIsInFlight(config:ConcreteConfiguration, gls:GLS_State) 
-    requires forall ep :: ep in gls.ls.servers <==> ep in config;
-    requires forall ep | ep in gls.ls.servers :: gls.ls.servers[ep].config == config;
+predicate OneTransferMessageIsInFlight(config:ConcreteConfiguration, gls:TimestampedGLS_State) 
+    requires forall ep :: ep in gls.tls.t_servers <==> ep in config;
+    requires forall ep | ep in gls.tls.t_servers :: gls.tls.t_servers[ep].v.config == config;
 {
     forall p1, p2 | IsInFlightTransferMessage(config, gls, p1) && IsInFlightTransferMessage(config, gls, p2) :: p1 == p2
 }
 
-predicate ZeroTransferMessageIsInFlight(config:ConcreteConfiguration, gls:GLS_State) 
-    requires forall ep :: ep in gls.ls.servers <==> ep in config;
-    requires forall ep | ep in gls.ls.servers :: gls.ls.servers[ep].config == config;
+predicate ZeroTransferMessageIsInFlight(config:ConcreteConfiguration, gls:TimestampedGLS_State) 
+    requires forall ep :: ep in gls.tls.t_servers <==> ep in config;
+    requires forall ep | ep in gls.tls.t_servers :: gls.tls.t_servers[ep].v.config == config;
 {
-    forall p | p in gls.ls.environment.sentPackets  :: ! IsInFlightTransferMessage(config, gls, p)
+    forall p | p in gls.tls.t_environment.sentPackets  :: ! IsInFlightTransferMessage(config, gls, p)
 }
 
-predicate NoLockHolderImpliesOneTransferMessageInFlight(config:ConcreteConfiguration, gls:GLS_State) 
-    requires forall ep :: ep in gls.ls.servers <==> ep in config;
-    requires forall ep | ep in gls.ls.servers :: gls.ls.servers[ep].config == config;
+predicate NoLockHolderImpliesOneTransferMessageInFlight(config:ConcreteConfiguration, gls:TimestampedGLS_State) 
+    requires forall ep :: ep in gls.tls.t_servers <==> ep in config;
+    requires forall ep | ep in gls.tls.t_servers :: gls.tls.t_servers[ep].v.config == config;
 {
     NoLockHolder(config, gls) ==> OneTransferMessageIsInFlight(config, gls)
 }   
 
-predicate AllTransferMessageInFlightHaveDstLastInHistory(config:ConcreteConfiguration, gls:GLS_State)
+predicate AllTransferMessageInFlightHaveDstLastInHistory(config:ConcreteConfiguration, gls:TimestampedGLS_State)
     requires |gls.history| > 0;
-    requires forall ep :: ep in gls.ls.servers <==> ep in config;
-    requires forall ep | ep in gls.ls.servers :: gls.ls.servers[ep].config == config;
+    requires forall ep :: ep in gls.tls.t_servers <==> ep in config;
+    requires forall ep | ep in gls.tls.t_servers :: gls.tls.t_servers[ep].v.config == config;
 {
     forall p | IsInFlightTransferMessage(config, gls, p) :: p.dst == gls.history[|gls.history|-1]
 }   
 
-predicate AllTransferMessageInFlightHaveEpochEqualsHistoryLength(config:ConcreteConfiguration, gls:GLS_State)
+predicate AllTransferMessageInFlightHaveEpochEqualsHistoryLength(config:ConcreteConfiguration, gls:TimestampedGLS_State)
     requires |gls.history| > 0;
-    requires forall ep :: ep in gls.ls.servers <==> ep in config;
-    requires forall ep | ep in gls.ls.servers :: gls.ls.servers[ep].config == config;
+    requires forall ep :: ep in gls.tls.t_servers <==> ep in config;
+    requires forall ep | ep in gls.tls.t_servers :: gls.tls.t_servers[ep].v.config == config;
 {
-    forall p | IsInFlightTransferMessage(config, gls, p) :: p.msg.transfer_epoch == |gls.history|
+    forall p | IsInFlightTransferMessage(config, gls, p) :: p.msg.v.transfer_epoch == |gls.history|
 }   
 
-predicate SomeLockHolderImpliesNoTransferMessageInFlight(config:ConcreteConfiguration, gls:GLS_State) 
-    requires forall ep :: ep in gls.ls.servers <==> ep in config;
-    requires forall ep | ep in gls.ls.servers :: gls.ls.servers[ep].config == config;
+predicate SomeLockHolderImpliesNoTransferMessageInFlight(config:ConcreteConfiguration, gls:TimestampedGLS_State) 
+    requires forall ep :: ep in gls.tls.t_servers <==> ep in config;
+    requires forall ep | ep in gls.tls.t_servers :: gls.tls.t_servers[ep].v.config == config;
 {
     !NoLockHolder(config, gls) ==> ZeroTransferMessageIsInFlight(config, gls)
 }   
 
-predicate SomeLockHolderImpliesEpochIsHistoryLength(config:ConcreteConfiguration, gls:GLS_State) 
-    requires forall ep :: ep in gls.ls.servers <==> ep in config;
-    requires forall ep | ep in gls.ls.servers :: gls.ls.servers[ep].config == config;
+predicate SomeLockHolderImpliesEpochIsHistoryLength(config:ConcreteConfiguration, gls:TimestampedGLS_State) 
+    requires forall ep :: ep in gls.tls.t_servers <==> ep in config;
+    requires forall ep | ep in gls.tls.t_servers :: gls.tls.t_servers[ep].v.config == config;
 {
-    forall h | h in config && gls.ls.servers[h].held :: gls.ls.servers[h].epoch == |gls.history|
+    forall h | h in config && gls.tls.t_servers[h].v.held :: gls.tls.t_servers[h].v.epoch == |gls.history|
 }   
 
-predicate SomeLockHolderImpliesHolderIsLastInHistory(config:ConcreteConfiguration, gls:GLS_State)
+predicate SomeLockHolderImpliesHolderIsLastInHistory(config:ConcreteConfiguration, gls:TimestampedGLS_State)
     requires |gls.history| > 0;
-    requires forall ep :: ep in gls.ls.servers <==> ep in config;
-    requires forall ep | ep in gls.ls.servers :: gls.ls.servers[ep].config == config;
+    requires forall ep :: ep in gls.tls.t_servers <==> ep in config;
+    requires forall ep | ep in gls.tls.t_servers :: gls.tls.t_servers[ep].v.config == config;
 {
-    forall ep | ep in config && gls.ls.servers[ep].held :: gls.history[|gls.history|-1] == ep
+    forall ep | ep in config && gls.tls.t_servers[ep].v.held :: gls.history[|gls.history|-1] == ep
 }
 
-lemma lemma_History_Length_Invariant(config:ConcreteConfiguration, glb:seq<GLS_State>)
-    requires |glb| > 0;
-    requires  GLS_Init(glb[0], config);
-    requires forall i {:trigger GLS_Next(glb[i], glb[i+1])} :: 0 <= i < |glb| - 1 ==>  GLS_Next(glb[i], glb[i+1]);
-    requires forall i | 0 <= i < |glb| :: (forall ep :: ep in glb[i].ls.servers <==> ep in config);
-    requires forall i | 0 <= i < |glb| :: (forall ep | ep in glb[i].ls.servers :: glb[i].ls.servers[ep].config == config);
-    ensures forall i | 0 <= i < |glb| :: SomeLockHolderImpliesEpochIsHistoryLength(config, glb[i]);
-    ensures forall i | 0 <= i < |glb| :: |glb[i].history| > 0;
-    ensures forall i | 0 <= i < |glb| :: HistoryLengthInvariant(config, glb[i]);
-{
-    // Base Case
-    assert glb[0].history == [config[0]];
-    assert glb[0].ls.servers[config[0]].epoch == 1;
-    assert HistoryLengthInvariant(config, glb[0]);
+// lemma lemma_History_Length_Invariant(config:ConcreteConfiguration, glb:seq<GLS_State>)
+//     requires |glb| > 0;
+//     requires  GLS_Init(glb[0], config);
+//     requires forall i {:trigger GLS_Next(glb[i], glb[i+1])} :: 0 <= i < |glb| - 1 ==>  GLS_Next(glb[i], glb[i+1]);
+//     requires forall i | 0 <= i < |glb| :: (forall ep :: ep in glb[i].ls.servers <==> ep in config);
+//     requires forall i | 0 <= i < |glb| :: (forall ep | ep in glb[i].ls.servers :: glb[i].ls.servers[ep].config == config);
+//     ensures forall i | 0 <= i < |glb| :: SomeLockHolderImpliesEpochIsHistoryLength(config, glb[i]);
+//     ensures forall i | 0 <= i < |glb| :: |glb[i].history| > 0;
+//     ensures forall i | 0 <= i < |glb| :: HistoryLengthInvariant(config, glb[i]);
+// {
+//     // Base Case
+//     assert glb[0].history == [config[0]];
+//     assert glb[0].ls.servers[config[0]].epoch == 1;
+//     assert HistoryLengthInvariant(config, glb[0]);
 
-    // Inductive Case
-    var i := 1;
-    while i < |glb| 
-        decreases |glb| - i;
-        invariant 1 <= i <= |glb|;
-        invariant forall k | 0 <= k < |glb|-1 :: GLS_Next(glb[k], glb[k+1]);
-        invariant forall k | 0 <= k < i :: |glb[k].history| > 0;
-        invariant forall k | 0 <= k < i :: HistoryLengthInvariant(config, glb[k]);
-    {
-        var k := i-1;
-        var gls, gls' := glb[k], glb[k+1];
-        assert HistoryLengthInvariant(config, gls);
+//     // Inductive Case
+//     var i := 1;
+//     while i < |glb| 
+//         decreases |glb| - i;
+//         invariant 1 <= i <= |glb|;
+//         invariant forall k | 0 <= k < |glb|-1 :: GLS_Next(glb[k], glb[k+1]);
+//         invariant forall k | 0 <= k < i :: |glb[k].history| > 0;
+//         invariant forall k | 0 <= k < i :: HistoryLengthInvariant(config, glb[k]);
+//     {
+//         var k := i-1;
+//         var gls, gls' := glb[k], glb[k+1];
+//         assert HistoryLengthInvariant(config, gls);
 
-        if !NoLockHolder(config, gls) {
-            // If someone holds the lock in state gls. 
-            // Then I know that there are no Transfer messages in flight in gls
-            lemma_History_Length_Invariant_Induction_A(config, gls, gls');
-        } else {
-            // If no one holds the lock in state gls. 
-            // Then I know that there is only one Transfer message in flight in gls
-            assert NoLockHolder(config, gls);
-            lemma_History_Length_Invariant_Induction_B(config, gls, gls');
-        }
-        i := i + 1; 
-    }
-}
+//         if !NoLockHolder(config, gls) {
+//             // If someone holds the lock in state gls. 
+//             // Then I know that there are no Transfer messages in flight in gls
+//             lemma_History_Length_Invariant_Induction_A(config, gls, gls');
+//         } else {
+//             // If no one holds the lock in state gls. 
+//             // Then I know that there is only one Transfer message in flight in gls
+//             assert NoLockHolder(config, gls);
+//             lemma_History_Length_Invariant_Induction_B(config, gls, gls');
+//         }
+//         i := i + 1; 
+//     }
+// }
 
-/* First branch of lemma_History_Length_Invariant proof, 
-* where !NoLockHolder(config, gls); */
-lemma lemma_History_Length_Invariant_Induction_A(config:ConcreteConfiguration, gls:GLS_State, gls':GLS_State)
-    requires forall ep :: ep in gls.ls.servers <==> ep in config;
-    requires forall ep | ep in gls.ls.servers :: gls.ls.servers[ep].config == config;
-    requires GLS_Next(gls, gls');
-    requires |gls.history| > 0
-    requires HistoryLengthInvariant(config, gls);
-    requires !NoLockHolder(config, gls);
-    ensures |gls'.history| > 0
-    ensures HistoryLengthInvariant(config, gls');
-{
-    assert ZeroTransferMessageIsInFlight(config, gls);
-    assert LS_Next(gls.ls, gls'.ls);
+// /* First branch of lemma_History_Length_Invariant proof, 
+// * where !NoLockHolder(config, gls); */
+// lemma lemma_History_Length_Invariant_Induction_A(config:ConcreteConfiguration, gls:TimestampedGLS_State, gls':GLS_State)
+//     requires forall ep :: ep in gls.ls.servers <==> ep in config;
+//     requires forall ep | ep in gls.ls.servers :: gls.ls.servers[ep].config == config;
+//     requires GLS_Next(gls, gls');
+//     requires |gls.history| > 0
+//     requires HistoryLengthInvariant(config, gls);
+//     requires !NoLockHolder(config, gls);
+//     ensures |gls'.history| > 0
+//     ensures HistoryLengthInvariant(config, gls');
+// {
+//     assert ZeroTransferMessageIsInFlight(config, gls);
+//     assert LS_Next(gls.ls, gls'.ls);
 
-    if (&& gls.ls.environment.nextStep.LEnvStepHostIos? 
-        && gls.ls.environment.nextStep.actor in gls.ls.servers) {
-        // If gls->gls' is a node Grant or Accept step
-        var id, ios := gls.ls.environment.nextStep.actor, gls.ls.environment.nextStep.ios;
-        assert NodeNext(gls.ls.servers[id], gls'.ls.servers[id], ios);
+//     if (&& gls.ls.environment.nextStep.LEnvStepHostIos? 
+//         && gls.ls.environment.nextStep.actor in gls.ls.servers) {
+//         // If gls->gls' is a node Grant or Accept step
+//         var id, ios := gls.ls.environment.nextStep.actor, gls.ls.environment.nextStep.ios;
+//         assert NodeNext(gls.ls.servers[id], gls'.ls.servers[id], ios);
 
-        if NodeGrant(gls.ls.servers[id], gls'.ls.servers[id], ios) {
-            assert HistoryLengthInvariant(config, gls');  // Dafny magic!
-        } else {
-            assert NodeAccept(gls.ls.servers[id], gls'.ls.servers[id], ios);
-            if ios[0].LIoOpTimeoutReceive? {
-                assert gls'.ls.servers == gls.ls.servers;
-                assert gls'.ls.environment.sentPackets == gls.ls.environment.sentPackets;
-            } else {
-                if (&& !gls.ls.servers[id].held
-                    && ios[0].r.src in gls.ls.servers[id].config
-                    && ios[0].r.msg.Transfer? 
-                    && ios[0].r.msg.transfer_epoch > gls.ls.servers[id].epoch
-                ) {
-                    assert ios[0].LIoOpReceive?;
-                    assert IsValidLIoOp(ios[0], id, gls.ls.environment);
-                    var m := ios[0].r;
-                    assert m in gls.ls.environment.sentPackets;
-                    assert m.dst == id; 
-                    assert false; // contradicts ZeroTransferMessageIsInFlight(config, gls)
-                } else {
-                    assert gls'.ls.servers == gls.ls.servers;
-                    assert gls'.ls.environment.sentPackets == gls.ls.environment.sentPackets;
-                }
-            }
-        }
-        assert HistoryLengthInvariant(config, gls');
-    } else {
-        // If gls->gls' is purely an environment step
-        assert gls.ls.servers == gls'.ls.servers && gls.history == gls'.history;
-        if !gls.ls.environment.nextStep.LEnvStepHostIos? {
-            match gls.ls.environment.nextStep {
-                case LEnvStepHostIos(actor, ios, nodestep) => assert false;
-                case LEnvStepDeliverPacket(p) => assert LEnvironment_Stutter(gls.ls.environment, gls'.ls.environment);
-                case LEnvStepAdvanceTime => assert LEnvironment_AdvanceTime(gls.ls.environment, gls'.ls.environment);
-                case LEnvStepStutter => assert LEnvironment_Stutter(gls.ls.environment, gls'.ls.environment);
-            }
-            assert gls'.ls.environment.sentPackets == gls.ls.environment.sentPackets;
-        } else {
-            assert gls.ls.environment.nextStep.actor !in gls.ls.servers;
-        }
-        assert HistoryLengthInvariant(config, gls');
-    }
-}
+//         if NodeGrant(gls.ls.servers[id], gls'.ls.servers[id], ios) {
+//             assert HistoryLengthInvariant(config, gls');  // Dafny magic!
+//         } else {
+//             assert NodeAccept(gls.ls.servers[id], gls'.ls.servers[id], ios);
+//             if ios[0].LIoOpTimeoutReceive? {
+//                 assert gls'.ls.servers == gls.ls.servers;
+//                 assert gls'.ls.environment.sentPackets == gls.ls.environment.sentPackets;
+//             } else {
+//                 if (&& !gls.ls.servers[id].held
+//                     && ios[0].r.src in gls.ls.servers[id].config
+//                     && ios[0].r.msg.Transfer? 
+//                     && ios[0].r.msg.transfer_epoch > gls.ls.servers[id].epoch
+//                 ) {
+//                     assert ios[0].LIoOpReceive?;
+//                     assert IsValidLIoOp(ios[0], id, gls.ls.environment);
+//                     var m := ios[0].r;
+//                     assert m in gls.ls.environment.sentPackets;
+//                     assert m.dst == id; 
+//                     assert false; // contradicts ZeroTransferMessageIsInFlight(config, gls)
+//                 } else {
+//                     assert gls'.ls.servers == gls.ls.servers;
+//                     assert gls'.ls.environment.sentPackets == gls.ls.environment.sentPackets;
+//                 }
+//             }
+//         }
+//         assert HistoryLengthInvariant(config, gls');
+//     } else {
+//         // If gls->gls' is purely an environment step
+//         assert gls.ls.servers == gls'.ls.servers && gls.history == gls'.history;
+//         if !gls.ls.environment.nextStep.LEnvStepHostIos? {
+//             match gls.ls.environment.nextStep {
+//                 case LEnvStepHostIos(actor, ios, nodestep) => assert false;
+//                 case LEnvStepDeliverPacket(p) => assert LEnvironment_Stutter(gls.ls.environment, gls'.ls.environment);
+//                 case LEnvStepAdvanceTime => assert LEnvironment_AdvanceTime(gls.ls.environment, gls'.ls.environment);
+//                 case LEnvStepStutter => assert LEnvironment_Stutter(gls.ls.environment, gls'.ls.environment);
+//             }
+//             assert gls'.ls.environment.sentPackets == gls.ls.environment.sentPackets;
+//         } else {
+//             assert gls.ls.environment.nextStep.actor !in gls.ls.servers;
+//         }
+//         assert HistoryLengthInvariant(config, gls');
+//     }
+// }
 
 
-/* Second branch of lemma_History_Length_Invariant proof, 
-* where NoLockHolder(config, gls); */
-lemma lemma_History_Length_Invariant_Induction_B(config:ConcreteConfiguration, gls:GLS_State, gls':GLS_State)
-    requires forall ep :: ep in gls.ls.servers <==> ep in config;
-    requires forall ep | ep in gls.ls.servers :: gls.ls.servers[ep].config == config;
-    requires GLS_Next(gls, gls');
-    requires |gls.history| > 0
-    requires HistoryLengthInvariant(config, gls);
-    requires NoLockHolder(config, gls);
-    ensures |gls'.history| > 0
-    ensures HistoryLengthInvariant(config, gls');
-{
-    assert OneTransferMessageIsInFlight(config, gls);
-    assert LS_Next(gls.ls, gls'.ls);
-    if (&& gls.ls.environment.nextStep.LEnvStepHostIos? 
-        && gls.ls.environment.nextStep.actor in gls.ls.servers) {
-        // If gls->gls' is a node Grant or Accept step
-        var id, ios := gls.ls.environment.nextStep.actor, gls.ls.environment.nextStep.ios;
-        assert id in config;
-        assert NodeNext(gls.ls.servers[id], gls'.ls.servers[id], ios);
+// /* Second branch of lemma_History_Length_Invariant proof, 
+// * where NoLockHolder(config, gls); */
+// lemma lemma_History_Length_Invariant_Induction_B(config:ConcreteConfiguration, gls:TimestampedGLS_State, gls':GLS_State)
+//     requires forall ep :: ep in gls.ls.servers <==> ep in config;
+//     requires forall ep | ep in gls.ls.servers :: gls.ls.servers[ep].config == config;
+//     requires GLS_Next(gls, gls');
+//     requires |gls.history| > 0
+//     requires HistoryLengthInvariant(config, gls);
+//     requires NoLockHolder(config, gls);
+//     ensures |gls'.history| > 0
+//     ensures HistoryLengthInvariant(config, gls');
+// {
+//     assert OneTransferMessageIsInFlight(config, gls);
+//     assert LS_Next(gls.ls, gls'.ls);
+//     if (&& gls.ls.environment.nextStep.LEnvStepHostIos? 
+//         && gls.ls.environment.nextStep.actor in gls.ls.servers) {
+//         // If gls->gls' is a node Grant or Accept step
+//         var id, ios := gls.ls.environment.nextStep.actor, gls.ls.environment.nextStep.ios;
+//         assert id in config;
+//         assert NodeNext(gls.ls.servers[id], gls'.ls.servers[id], ios);
 
-        if NodeGrant(gls.ls.servers[id], gls'.ls.servers[id], ios) {
-            if gls.ls.servers[id].held && gls.ls.servers[id].epoch < 0xFFFF_FFFF_FFFF_FFFF {
-                assert false;  // contradics NoLockHolder(config, gls);
-            } else {
-                assert gls'.ls.servers == gls.ls.servers;
-                assert gls'.ls.environment.sentPackets == gls.ls.environment.sentPackets;
-            }
-        } else {
-            assert NodeAccept(gls.ls.servers[id], gls'.ls.servers[id], ios);
-            if ios[0].LIoOpTimeoutReceive? {
-                assert gls'.ls.servers == gls.ls.servers;
-                assert gls'.ls.environment.sentPackets == gls.ls.environment.sentPackets;
-            } else {
-                if (!gls.ls.servers[id].held 
-                    && ios[0].r.src in gls.ls.servers[id].config
-                    && ios[0].r.msg.Transfer? 
-                    && ios[0].r.msg.transfer_epoch > gls.ls.servers[id].epoch)
-                {
-                    assert gls'.ls.servers[id].held;
-                    assert !NoLockHolder(config, gls');
-                    assert forall id' | id' in config && id' != id :: !gls.ls.servers[id'].held;
-                    forall p | p in gls'.ls.environment.sentPackets  
-                    ensures !IsInFlightTransferMessage(config, gls', p)
-                    {
-                        if p.dst in config && p.src in config && p.msg.Transfer? {
-                            assert p in gls.ls.environment.sentPackets;
-                            if p.dst == id {
-                                if p.msg.transfer_epoch > gls.ls.servers[id].epoch {
-                                    var receivedMessage := ios[0].r;
-                                    assert IsValidLIoOp(ios[0], id, gls.ls.environment);
-                                    assert receivedMessage.dst == id;
-                                    assert IsInFlightTransferMessage(config, gls, receivedMessage);
-                                    assert IsInFlightTransferMessage(config, gls, p);
-                                    assert p == receivedMessage;
-                                    assert p.msg.transfer_epoch == gls'.ls.servers[id].epoch;
-                                    assert !IsInFlightTransferMessage(config, gls', p);
-                                } else {
-                                    assert !IsInFlightTransferMessage(config, gls', p);
-                                }
-                            } else {
-                                assert gls'.ls.servers[p.dst].epoch == gls.ls.servers[p.dst].epoch;
-                                assert gls.ls.servers[p.dst].epoch >= p.msg.transfer_epoch;
-                            }
-                        }
-                    }
-                    assert HistoryLengthInvariant(config, gls');  // Dafny magic!
-                } else {
-                    assert gls'.ls.servers == gls.ls.servers;
-                    assert gls'.ls.environment.sentPackets == gls.ls.environment.sentPackets;
-                }
-            }
-        }
-        assert HistoryLengthInvariant(config, gls');
-    } else {
-        // If gls->gls' is purely an environment step
-        // (not gls.ls.environment.nextStep.LEnvStepHostIos?) or (not gls.ls.environment.nextStep.actor in gls.ls.servers)
-        assert gls.ls.servers == gls'.ls.servers && gls.history == gls'.history;
-        if !gls.ls.environment.nextStep.LEnvStepHostIos? {
-            match gls.ls.environment.nextStep {
-                case LEnvStepHostIos(actor, ios, nodestep) => assert false;
-                case LEnvStepDeliverPacket(p) => assert LEnvironment_Stutter(gls.ls.environment, gls'.ls.environment);
-                case LEnvStepAdvanceTime => assert LEnvironment_AdvanceTime(gls.ls.environment, gls'.ls.environment);
-                case LEnvStepStutter => assert LEnvironment_Stutter(gls.ls.environment, gls'.ls.environment);
-            }
-            assert gls'.ls.environment.sentPackets == gls.ls.environment.sentPackets;
-        } else {
-            assert gls.ls.environment.nextStep.actor !in gls.ls.servers;
-            if gls.ls.environment.nextStep.LEnvStepHostIos? {  
-                // Any message sent in this step cannot be classified as InFlight 
-                // because their source == actor is not in config
-                assert OneTransferMessageIsInFlight(config, gls);
-                var id, ios := gls.ls.environment.nextStep.actor, gls.ls.environment.nextStep.ios;
-                forall io | io in ios && io.LIoOpSend?
-                ensures !IsInFlightTransferMessage(config, gls', io.s)
-                {}
-                assert gls'.ls.environment.sentPackets == gls.ls.environment.sentPackets + (set io | io in ios && io.LIoOpSend? :: io.s);
-                assert forall p | p in gls'.ls.environment.sentPackets && IsInFlightTransferMessage(config, gls', p) :: p in gls.ls.environment.sentPackets;
-                assert NoLockHolder(config, gls');
-                assert OneTransferMessageIsInFlight(config, gls');
-            } else {
-                assert gls'.ls.environment.sentPackets == gls.ls.environment.sentPackets;
-            }
-        }
-        assert HistoryLengthInvariant(config, gls');
-    }
-}
+//         if NodeGrant(gls.ls.servers[id], gls'.ls.servers[id], ios) {
+//             if gls.ls.servers[id].held && gls.ls.servers[id].epoch < 0xFFFF_FFFF_FFFF_FFFF {
+//                 assert false;  // contradics NoLockHolder(config, gls);
+//             } else {
+//                 assert gls'.ls.servers == gls.ls.servers;
+//                 assert gls'.ls.environment.sentPackets == gls.ls.environment.sentPackets;
+//             }
+//         } else {
+//             assert NodeAccept(gls.ls.servers[id], gls'.ls.servers[id], ios);
+//             if ios[0].LIoOpTimeoutReceive? {
+//                 assert gls'.ls.servers == gls.ls.servers;
+//                 assert gls'.ls.environment.sentPackets == gls.ls.environment.sentPackets;
+//             } else {
+//                 if (!gls.ls.servers[id].held 
+//                     && ios[0].r.src in gls.ls.servers[id].config
+//                     && ios[0].r.msg.Transfer? 
+//                     && ios[0].r.msg.transfer_epoch > gls.ls.servers[id].epoch)
+//                 {
+//                     assert gls'.ls.servers[id].held;
+//                     assert !NoLockHolder(config, gls');
+//                     assert forall id' | id' in config && id' != id :: !gls.ls.servers[id'].held;
+//                     forall p | p in gls'.ls.environment.sentPackets  
+//                     ensures !IsInFlightTransferMessage(config, gls', p)
+//                     {
+//                         if p.dst in config && p.src in config && p.msg.Transfer? {
+//                             assert p in gls.ls.environment.sentPackets;
+//                             if p.dst == id {
+//                                 if p.msg.transfer_epoch > gls.ls.servers[id].epoch {
+//                                     var receivedMessage := ios[0].r;
+//                                     assert IsValidLIoOp(ios[0], id, gls.ls.environment);
+//                                     assert receivedMessage.dst == id;
+//                                     assert IsInFlightTransferMessage(config, gls, receivedMessage);
+//                                     assert IsInFlightTransferMessage(config, gls, p);
+//                                     assert p == receivedMessage;
+//                                     assert p.msg.transfer_epoch == gls'.ls.servers[id].epoch;
+//                                     assert !IsInFlightTransferMessage(config, gls', p);
+//                                 } else {
+//                                     assert !IsInFlightTransferMessage(config, gls', p);
+//                                 }
+//                             } else {
+//                                 assert gls'.ls.servers[p.dst].epoch == gls.ls.servers[p.dst].epoch;
+//                                 assert gls.ls.servers[p.dst].epoch >= p.msg.transfer_epoch;
+//                             }
+//                         }
+//                     }
+//                     assert HistoryLengthInvariant(config, gls');  // Dafny magic!
+//                 } else {
+//                     assert gls'.ls.servers == gls.ls.servers;
+//                     assert gls'.ls.environment.sentPackets == gls.ls.environment.sentPackets;
+//                 }
+//             }
+//         }
+//         assert HistoryLengthInvariant(config, gls');
+//     } else {
+//         // If gls->gls' is purely an environment step
+//         // (not gls.ls.environment.nextStep.LEnvStepHostIos?) or (not gls.ls.environment.nextStep.actor in gls.ls.servers)
+//         assert gls.ls.servers == gls'.ls.servers && gls.history == gls'.history;
+//         if !gls.ls.environment.nextStep.LEnvStepHostIos? {
+//             match gls.ls.environment.nextStep {
+//                 case LEnvStepHostIos(actor, ios, nodestep) => assert false;
+//                 case LEnvStepDeliverPacket(p) => assert LEnvironment_Stutter(gls.ls.environment, gls'.ls.environment);
+//                 case LEnvStepAdvanceTime => assert LEnvironment_AdvanceTime(gls.ls.environment, gls'.ls.environment);
+//                 case LEnvStepStutter => assert LEnvironment_Stutter(gls.ls.environment, gls'.ls.environment);
+//             }
+//             assert gls'.ls.environment.sentPackets == gls.ls.environment.sentPackets;
+//         } else {
+//             assert gls.ls.environment.nextStep.actor !in gls.ls.servers;
+//             if gls.ls.environment.nextStep.LEnvStepHostIos? {  
+//                 // Any message sent in this step cannot be classified as InFlight 
+//                 // because their source == actor is not in config
+//                 assert OneTransferMessageIsInFlight(config, gls);
+//                 var id, ios := gls.ls.environment.nextStep.actor, gls.ls.environment.nextStep.ios;
+//                 forall io | io in ios && io.LIoOpSend?
+//                 ensures !IsInFlightTransferMessage(config, gls', io.s)
+//                 {}
+//                 assert gls'.ls.environment.sentPackets == gls.ls.environment.sentPackets + (set io | io in ios && io.LIoOpSend? :: io.s);
+//                 assert forall p | p in gls'.ls.environment.sentPackets && IsInFlightTransferMessage(config, gls', p) :: p in gls.ls.environment.sentPackets;
+//                 assert NoLockHolder(config, gls');
+//                 assert OneTransferMessageIsInFlight(config, gls');
+//             } else {
+//                 assert gls'.ls.environment.sentPackets == gls.ls.environment.sentPackets;
+//             }
+//         }
+//         assert HistoryLengthInvariant(config, gls');
+//     }
+// }
 }
